empty message

isabelleSrc/P02.thy
@@ -1,29 +1,59 @@
-theory P02
+theory P02 
 imports Main 
 begin 
-(*from now on I will mix isar and apply-script proofs and I will also mix step-by-step solving with automation*)
-(*find the last but one element of a list*)
 
-
-(*using a default element in case the list is too small*)
-fun p02_1 :: "'a list \<Rightarrow> 'a \<Rightarrow> 'a" where
+fun p02_1 :: "'a list \<Rightarrow> 'a  \<Rightarrow> 'a" where 
 "p02_1 [] def = def"|
-"p02_1 (x#xs) def = (case xs of  [y] \<Rightarrow> x | _  \<Rightarrow>  p02_1 xs def) "
-
+"p02_1 [x] def = def"|
+"p02_1 [x , y] def = x"|
+"p02_1 (x#xs) def = p02_1 xs def"
 
 value "p02_1 [] 5 :: int"
-value "p02_1 [1] 7 :: int"
-value "p02_1 [1,2,3,4,5] 6 :: int"
+
+value "(p02_1 [2] 6) :: int"
+
+value "p02_1 [1,2] 3 :: int"
+
+lemma "p02_1 (xs @ [a , b]) def = a"
+proof (induct xs)
+  show "p02_1 ([] @ [a, b]) def = a" by simp
+ next 
+  fix aa xs 
+  show "p02_1 (xs @ [a, b]) def = a \<Longrightarrow> p02_1 ((aa # xs) @ [a, b]) def = a "
+  proof (cases xs)
+    assume "xs = []"
+    thus " p02_1 ((aa # xs) @ [a, b]) def = a" by simp
+   next
+    fix ab list 
+    assume a:" p02_1 (xs @ [a, b]) def = a" 
+    assume "xs = ab # list"
+    from this and a show "p02_1 ((aa # xs) @ [a, b]) def = a " 
+    proof (cases list)
+      assume " xs = ab # list"
+     moreover
+      assume " p02_1 (xs @ [a, b]) def = a"
+     moreover
+      assume "list = []"
+     ultimately
+      show "p02_1 ((aa # xs) @ [a, b]) def = a" by simp
+     next 
+      fix ac lista
+      assume " xs = ab # list"
+     moreover
+      assume "p02_1 (xs @ [a, b]) def = a"
+     moreover
+      assume "list = ac # lista"
+     ultimately
+      show "p02_1 ((aa # xs) @ [a, b]) def = a" by simp
+    qed
+  qed
+qed
 
 
-theorem tp02_1_1 : "p02_1 [] a = a" by auto
 
-theorem tp02_1_2 : "p02_1 [] a = a"
-using [[simp_trace_new mode=full]]
-apply (subst p02_1.simps)
-apply (rule refl)
-done 
 
-theorem isar_tp02_1_1 : "p02_1 [x] a = a" 
-proof - 
-have 
+fun p02_2 :: "'a list \<Rightarrow> 'a option" where 
+"p02_2 [] = None"|
+"p02_2 [x] = None"|
+"p02_2 [x,y] = Some x"|
+"p02_2 (x#xs) = p02_2 xs"
