OldisabelleSrc/P01.thy
@@ -1,0 +1,266 @@
+theory P01 
+imports Main 
+begin
+
+
+(*
+useful commands
+using [[simp_trace]] shows the used rewrite rules and what has been rewritten in the output tab
+using [[simp_trace_new]] only shows the rewrites in a new window
+using [[simp_trace_new mode=full]] shows the used rewrite rules and what has been rewritten
+simp only: <rule name> only uses one simplification rule and some trivial simplifications
+subst really only uses one simplification rule
+
+how to typecast :  int (5::nat)  ==  (5::int) (write for example int like a function \<longrightarrow> int (value))
+*)
+
+
+(*using a default value*)
+fun p01_1 ::  "'a list \<Rightarrow> 'a \<Rightarrow> 'a" where 
+"p01_1 [] def = def"|
+"p01_1 [x] _ = x"|
+"p01_1 (x#xs) def = p01_1 xs def" 
+
+(*evaluate an expression*)
+value "p01_1 [1,2,3,4] 5 :: int" 
+value "p01_1 [] 5 :: int"
+
+(*show the type of an expression*)
+term p01_1
+
+(*show the definition of a theorem*)
+thm p01_1.simps(1)
+thm append_Nil
+
+theorem tp01_1_1 : "p01_1 [] a = a"
+apply (rule p01_1.simps(1)) 
+done 
+
+
+theorem isar_tp01_1_1 :"p01_1 [] a = a"
+proof - 
+  show ?thesis by (rule p01_1.simps(1))
+qed 
+
+
+theorem tp01_1_2 : "p01_1 ( ls @ [a]) b = a "
+apply (induct "ls")
+apply simp
+apply (case_tac "ls @ [a]")
+apply simp
+apply simp
+done
+
+
+(*step by step rewriting*)
+theorem tp01_1_4 : "p01_1 (ls @ [a]) b = a"
+apply (induct "ls")
+  apply (subst append.append_Nil)
+  apply (subst p01_1.simps(2))
+  apply (rule refl)
+apply (case_tac ls)
+(*case ls = []*)
+  apply (erule_tac ?t = ls and ?s = "[]" in  ssubst)
+  apply (subst append.append_Cons)
+  apply (subst append.append_Nil)
+  apply (subst  p01_1.simps(3))
+  apply (subst p01_1.simps(2))
+  apply (rule refl)
+(*case ls = aaa # list*)
+  apply (rule_tac ?t = ls and ?s = "aaa # list" in ssubst)
+  apply assumption
+  apply (rule_tac ?t = ls and ?s = "aaa # list" in ssubst)
+  apply assumption
+  apply (subst  append.append_Cons)+ (*the "+" means that we apply the same rule as often as possible*)
+  apply (subst p01_1.simps(3))
+  apply hypsubst
+  apply (subst (asm) append.append_Cons)
+  apply (assumption)
+done
+ 
+
+
+(*isar proof using automation*)
+theorem isar_tp01_1_2 : "p01_1 ( ls @ [a]) b = a "
+proof (induction ls)
+{
+  show " p01_1 ([] @ [a]) b = a" by simp
+}
+{
+  fix aa ls
+  show " p01_1 (ls @ [a]) b = a \<Longrightarrow> p01_1 ((aa # ls) @ [a]) b = a " 
+  proof (cases ls)
+  {
+    show " p01_1 (ls @ [a]) b = a \<Longrightarrow> ls = [] \<Longrightarrow> p01_1 ((aa # ls) @ [a]) b = a" by simp
+    fix ab list
+    show "p01_1 (ls @ [a]) b = a \<Longrightarrow> ls = ab # list \<Longrightarrow> p01_1 ((aa # ls) @ [a]) b = a " by simp
+  }
+  qed
+}
+qed
+
+
+
+
+(*step by step syntactical replacement with Isar*)
+theorem isar_tp01_1_3 : fixes ls a b  shows "p01_1 ( ls @ [a]) b = a " 
+proof (induct ls)
+ case Nil
+  have "p01_1 ([] @ [a]) b =  p01_1 [a] b" unfolding append_Nil ..  (*instead of   the two dots ".." one could write "by (rule refl)" *)(*instead of unfolding \<rightarrow> "by (subst append_Nil[where ?ys = "[a]"]; rule refl)" *)
+  also have "\<dots> = a" unfolding p01_1.simps(2) ..
+  finally show "p01_1 ([] @ [a]) b = a" . 
+next
+ case (Cons  aa ls)
+  show " p01_1 (ls @ [a]) b = a \<Longrightarrow>  p01_1 ((aa # ls) @ [a]) b = a "
+  proof (cases ls)
+   case Nil
+    assume "ls = []" 
+    assume "p01_1 (ls @ [a]) b = a"
+    have " p01_1 ((aa # ls) @ [a]) b =  p01_1 (aa # ls @ [a]) b " unfolding append_Cons ..
+    also have "\<dots> = p01_1 (aa # [] @ [a]) b" unfolding \<open>ls = []\<close> ..
+    also have "\<dots> = p01_1 (aa # [a]) b" unfolding append_Nil ..
+    also have "\<dots> = p01_1 [a] b" unfolding p01_1.simps(3) ..
+    also have "\<dots> = a" unfolding p01_1.simps(2)  ..
+    finally show "p01_1 ((aa # ls) @ [a]) b = a" . 
+  next  
+   case (Cons ab list)
+    fix ab list 
+    assume IH:"p01_1 (ls @ [a]) b = a"
+    assume "ls = ab # list"
+
+    from  \<open>ls= ab # list\<close> and  IH have "p01_1 ((ab # list) @ [a]) b = a"  by (rule subst)
+    with append_Cons have  "p01_1 (ab # list @ [a]) b = a" by (rule subst)
+    note IH2 = this
+
+    have  "p01_1 ((aa # ls) @ [a]) b = p01_1 ((aa # ab # list)@ [a]) b" unfolding \<open>ls = ab # list\<close> ..
+    also have "\<dots> =  p01_1 (aa # (ab # list)@ [a]) b " unfolding append_Cons ..
+    also have "\<dots> =  p01_1 (aa # ab # list@ [a]) b" unfolding append_Cons ..
+    also have "\<dots> = p01_1 (ab # list @ [a]) b " unfolding p01_1.simps(3) ..
+    also have "\<dots> = a " unfolding IH2 ..
+    finally show " p01_1 ((aa # ls) @ [a]) b = a" .
+  qed
+qed
+
+
+(*on other way to proof this (a bit nonsensical ... )*)
+theorem isar_tp01_1_4 : fixes ls a b  shows "p01_1 ( ls @ [a]) b = a " 
+proof (induct ls)
+{
+  show "p01_1 ([] @ [a]) b = a"
+  proof (subst append_Nil)
+  {
+    show " p01_1 [a] b = a"
+    proof (subst p01_1.simps(2))
+    {
+      show "a = a" by (rule refl)
+    }
+    qed
+  }
+  qed
+  fix aa ls
+  assume "p01_1 (ls @ [a]) b = a"
+  show " p01_1 ((aa # ls) @ [a]) b = a "
+  proof (cases ls)
+  {
+    assume "ls = []"
+    show "p01_1 ((aa # ls) @ [a]) b = a"
+    proof (subst \<open>ls=[]\<close>)
+    {
+      show "p01_1 ([aa] @ [a]) b = a"
+      proof (subst append_Cons)
+      {
+        show "p01_1 (aa # [] @ [a]) b = a"
+        proof (subst append_Nil)
+        {
+          show " p01_1 [aa, a] b = a"
+          proof (subst p01_1.simps(3))
+          {
+            show "p01_1 [a] b = a" 
+            proof (subst p01_1.simps(2))
+            {
+              show "a = a" by (rule refl)
+            }
+            qed
+          }
+          qed
+        }
+        qed
+      }
+      qed
+    }
+    qed
+  }
+  fix ab list
+  assume "ls = ab # list"
+  from this and  \<open>p01_1 (ls @ [a]) b = a\<close> have "p01_1 ((ab # list) @ [a]) b = a" by (rule subst) 
+  with append_Cons have "p01_1 (ab # list @ [a]) b = a" by (rule subst)
+  show "p01_1 ((aa # ls) @ [a]) b = a" 
+  proof (subst \<open>ls = ab # list\<close>)
+  {
+    show " p01_1 ((aa # ab # list) @ [a]) b = a "
+    proof (subst  append_Cons)
+    {
+      show "p01_1 (aa # (ab # list) @ [a]) b = a "
+      proof (subst append_Cons )
+      {
+        show "p01_1 (aa # ab # list @ [a]) b = a "
+        proof (subst p01_1.simps(3))
+        {
+          show "p01_1 (ab # list @ [a]) b = a " by (rule \<open>p01_1 (ab # list @ [a]) b = a\<close>)
+        }
+        qed
+      }
+      qed
+    }
+    qed
+  }
+  qed
+  qed
+}
+qed
+
+
+
+
+find_theorems "(?x \<noteq> ?x) = False"
+lemma "p01_1 ls a \<noteq> a \<Longrightarrow> ls \<noteq> Nil"
+using [[simp_trace_new mode=full]] 
+proof (induct ls)
+ case Nil
+  assume "p01_1 [] a \<noteq> a"
+  hence "a \<noteq> a" unfolding p01_1.simps(1) ..
+  hence "\<not>(True)" unfolding simp_thms by (rule FalseE) (*the usage of simp_thms is discourage , use simp instead. I just want to show how this works*)
+  hence "False" unfolding simp_thms by (rule FalseE)
+  thus ?case by (rule FalseE)
+ next 
+  fix aa ls
+  assume "(p01_1 ls a \<noteq> a \<Longrightarrow> ls \<noteq> [])"
+  show "\<And>aa ls. (p01_1 ls a \<noteq> a \<Longrightarrow> ls \<noteq> []) \<Longrightarrow> p01_1 (aa # ls) a \<noteq> a \<Longrightarrow> aa # ls \<noteq> []" by auto
+  thm list.distinct(2)
+
+(*from now on I will mix isar and apply-script proofs and I will also mix step-by-step solving with automation*)
+
+
+fun p01_2 :: "'a list \<Rightarrow> 'a option" where
+"p01_2 [] = None"|
+"p01_2 [x] = Some x"|
+"p01_2 (x#xs) = p01_2 xs"
+
+
+value "p01_2 [1,2,3,4,5] :: int option"
+value "p01_2 [] :: int option"
+
+term p01_2
+
+
+lemma tp01_2_1 : "p01_2 [] = None"
+apply (rule p01_2.simps(1))
+done 
+
+lemma  isar_tp01_2_1 : "p01_2 [] = None"
+proof -
+show ?thesis by (rule p01_2.simps(1))
+qed
+
+
+lemma 
