OldisabelleSrc/P02.thy
@@ -1,0 +1,44 @@
+theory P02
+imports Main 
+begin 
+(*from now on I will mix isar and apply-script proofs and I will also mix step-by-step solving with automation*)
+(*find the last but one element of a list*)
+
+
+(*using a default element in case the list is too small*)
+fun p02_1 :: "'a list \<Rightarrow> 'a \<Rightarrow> 'a" where
+"p02_1 [] def = def"|
+"p02_1 (x#xs) def = (case xs of  [y] \<Rightarrow> x | _  \<Rightarrow>  p02_1 xs def) "
+
+
+value "p02_1 [] 5 :: int"
+value "p02_1 [1] 7 :: int"
+value "p02_1 [1,2,3,4,5] 6 :: int"
+
+
+theorem tp02_1_1 : "p02_1 [] a = a" by auto
+
+theorem tp02_1_2 : "p02_1 [] a = a"
+using [[simp_trace_new mode=full]]
+apply (subst p02_1.simps)
+apply (rule refl)
+done 
+
+theorem isar_tp02_1_1 : "p02_1 [x] a = a" 
+using [[simp_trace_new mode=full]]
+proof - 
+show ?thesis by (subst p02_1.simps(2); subst list.case(1); subst p02_1.simps(1); rule refl)
+qed
+
+theorem isar_tp02_1_2 : "length ls < 2 \<Longrightarrow> p02_1 ls a = a"
+proof (induct ls)
+  case Nil 
+  assume "length [] < 2"
+  show "p02_1 [] a = a"  by (subst p02_1.simps(1) ; rule refl)
+ next
+  case (Cons aa ls)
+  fix aa ls
+  assume "(length ls < 2 \<Longrightarrow> p02_1 ls a = a)"
+  assume "length (aa # ls) < 2"
+  
+  show " \<And>aa ls. (length ls < 2 \<Longrightarrow> p02_1 ls a = a) \<Longrightarrow> length (aa # ls) < 2 \<Longrightarrow> p02_1 (aa # ls) a = a" by auto
