OldisabelleSrc/P03.thy
@@ -1,0 +1,45 @@
+theory P03
+imports Main 
+begin 
+
+thm notE
+lemma "n = 0 \<Longrightarrow> n \<noteq> 0 \<Longrightarrow> n = 3" by (rule notE)
+using [[simp_trace_new mode=full]]
+proof - 
+assume a: "n = 0"
+assume b: "n \<noteq> 0"
+from a b have False by (simp )
+from a and b have "0 \<noteq> 0" by simp
+
+thm simp_thms
+fun p03_2 :: "'a list \<Rightarrow> nat \<Rightarrow> 'a option " where
+"p03_2 [] _ = None"|
+"p03_2 (x#xs) n = (if n = 1 then Some x else  p03_2 xs (n -1))"
+
+value  "p03_2 [1,2,3,4] 3 :: int option"
+
+
+lemma "p03_2 [] n = None"
+proof -
+  show ?thesis by (subst p03_2.simps(1); rule refl)
+qed
+thm subst
+lemma "p03_2 [x] 1  = Some x" by simp
+
+thm
+lemma " length ls  \<ge> n  \<Longrightarrow> n \<noteq> 0 \<Longrightarrow> p03_2 ls n = Some a"
+using [[simp_trace_new mode=full]]
+proof (induct ls)
+ case Nil
+  assume a:"\<not>(n = 0)"
+  assume "n \<le> length []"
+  with list.size(3) have "n \<le> 0" by (rule subst) 
+  with le_0_eq have "n = 0"  by (rule subst)
+  with a show "p03_2 [] n = Some a"  by (rule notE)
+ next
+show "\<And>aa ls. (n \<le> length ls \<Longrightarrow> n \<noteq> 0 \<Longrightarrow> p03_2 ls n = Some a) \<Longrightarrow> n \<le> length (aa # ls) \<Longrightarrow> n \<noteq> 0 \<Longrightarrow> p03_2 (aa # ls) n = Some a" by auto
+  fix aa ls
+  assume "n \<le> length ls \<Longrightarrow> n \<noteq> 0 \<Longrightarrow> p03_2 ls n = Some a"
+  assume " n \<le> length (aa # ls)"
+  assume "n \<noteq> 0"
+  
