isabelleSrc/P01.thy
@@ -1,268 +1,138 @@
 theory P01 
 imports Main 
-begin
+begin 
 
 
-(*
-useful commands
-using [[simp_trace]] shows the used rewrite rules and what has been rewritten in the output tab
-using [[simp_trace_new]] only shows the rewrites in a new window
-using [[simp_trace_new mode=full]] shows the used rewrite rules and what has been rewritten
-simp only: <rule name> only uses one simplification rule and some trivial simplifications
-subst really only uses one simplification rule
-*)
 
-
-(*using a default value*)
-fun p01_1 ::  "'a list \<Rightarrow> 'a \<Rightarrow> 'a" where 
+fun p01_1 :: "'a list \<Rightarrow> 'a \<Rightarrow> 'a" where 
 "p01_1 [] def = def"|
 "p01_1 [x] _ = x"|
-"p01_1 (x#xs) def = p01_1 xs def" 
+"p01_1 (x#xs) def = p01_1 xs def"
 
-(*evaluate an expression*)
-value "p01_1 [1,2,3,4] 5 :: int" 
+
 value "p01_1 [] 5 :: int"
 
-(*show the type of an expression*)
 term p01_1
 
-(*show the definition of a theorem*)
-thm p01_1.simps(1)
-thm append_Nil
 
-theorem tp01_1_1 : "p01_1 [] a = a"
-apply (rule p01_1.simps(1)) 
-done 
+lemma "p01_1 [] def = def" by simp 
+
+lemma "p01_1 [x] def = x" by simp
+
+lemma "p01_1 (xs @ [x]) def = x"
+proof (induct xs)
+  case Nil 
+  show ?case by simp
+ next 
+  fix a xs
+  show " p01_1 (xs @ [x]) def = x \<Longrightarrow> p01_1 ((a # xs) @ [x]) def = x "
+  proof (induct xs)
+    case Nil 
+    show ?case by simp
+   next 
+    fix aa xs 
+    assume "(p01_1 (xs @ [x]) def = x \<Longrightarrow> p01_1 ((a # xs) @ [x]) def = x)"
+    show "p01_1 ((aa # xs) @ [x]) def = x \<Longrightarrow> p01_1 ((a # aa # xs) @ [x]) def = x " by simp
+  qed
+qed
 
 
-theorem isar_tp01_1_1 :"p01_1 [] a = a"
-proof - 
-  show ?thesis by (rule p01_1.simps(1))
-qed 
 
 
-theorem tp01_1_2 : "p01_1 ( ls @ [a]) b = a "
-apply (induct "ls")
-apply simp
-apply (case_tac "ls @ [a]")
-apply simp
-apply simp
-done
+lemma "length xs \<ge> 1 \<Longrightarrow> p01_1 xs def = last xs"  
+proof (induct xs)
+  show "1 \<le> length [] \<Longrightarrow> p01_1 [] def = last []" by simp
+ next
+  fix xs a
+  show "(1 \<le> length xs \<Longrightarrow> p01_1 xs def = last xs) \<Longrightarrow> 1 \<le> length (a # xs) \<Longrightarrow> p01_1 (a # xs) def = last (a # xs)"
+  proof (cases xs)
+  show "(1 \<le> length xs \<Longrightarrow> p01_1 xs def = last xs) \<Longrightarrow> 1 \<le> length (a # xs) \<Longrightarrow> xs = [] \<Longrightarrow> p01_1 (a # xs) def = last (a # xs)" by simp
+ next
+  fix aa list
+  show " (1 \<le> length xs \<Longrightarrow> p01_1 xs def = last xs) \<Longrightarrow> 1 \<le> length (a # xs) \<Longrightarrow> xs = aa # list \<Longrightarrow> p01_1 (a # xs) def = last (a # xs)" by simp
+ qed
+qed
+  
 
-
-(*step by step rewriting*)
-theorem tp01_1_4 : "p01_1 (ls @ [a]) b = a"
-apply (induct "ls")
-  apply (subst append.append_Nil)
-  apply (subst p01_1.simps(2))
-  apply (rule refl)
-apply (case_tac ls)
-(*case ls = []*)
-  apply (erule_tac ?t = ls and ?s = "[]" in  ssubst)
-  apply (subst append.append_Cons)
-  apply (subst append.append_Nil)
-  apply (subst  p01_1.simps(3))
-  apply (subst p01_1.simps(2))
-  apply (rule refl)
-(*case ls = aaa # list*)
-  apply (rule_tac ?t = ls and ?s = "aaa # list" in ssubst)
-  apply assumption
-  apply (rule_tac ?t = ls and ?s = "aaa # list" in ssubst)
-  apply assumption
-  apply (subst  append.append_Cons)+ (*the "+" means that we apply the same rule as often as possible*)
-  apply (subst p01_1.simps(3))
-  apply hypsubst
-  apply (subst (asm) append.append_Cons)
-  apply (assumption)
-done
  
 
-
-(*isar proof using automation*)
-theorem isar_tp01_1_2 : "p01_1 ( ls @ [a]) b = a "
-proof (induction ls)
-{
-  show " p01_1 ([] @ [a]) b = a" by simp
-}
-{
-  fix aa ls
-  show " p01_1 (ls @ [a]) b = a \<Longrightarrow> p01_1 ((aa # ls) @ [a]) b = a " 
-  proof (cases ls)
-  {
-    show " p01_1 (ls @ [a]) b = a \<Longrightarrow> ls = [] \<Longrightarrow> p01_1 ((aa # ls) @ [a]) b = a" by simp
-    fix ab list
-    show "p01_1 (ls @ [a]) b = a \<Longrightarrow> ls = ab # list \<Longrightarrow> p01_1 ((aa # ls) @ [a]) b = a " by simp
-  }
-  qed
-}
+lemma "length xs \<ge> 1 \<Longrightarrow> p01_1 xs def = x \<Longrightarrow> x \<in> set xs" 
+proof (induct xs) 
+  show " 1 \<le> length [] \<Longrightarrow> p01_1 [] def = x \<Longrightarrow> x \<in> set []" by simp
+ next 
+  fix a xs 
+  show "(1 \<le> length xs \<Longrightarrow> p01_1 xs def = x \<Longrightarrow> x \<in> set xs) \<Longrightarrow> 1 \<le> length (a # xs) \<Longrightarrow> p01_1 (a # xs) def = x \<Longrightarrow> x \<in> set (a # xs) "
+  proof (cases xs)
+  assume "(1 \<le> length xs \<Longrightarrow> p01_1 xs def = x \<Longrightarrow> x \<in> set xs) "
+  assume " 1 \<le> length (a # xs)"
+  assume a:"xs = []"
+  assume " p01_1 (a # xs) def = x"
+  from this and a show "x \<in> set (a # xs)" by simp
+ next 
+  fix aa list 
+  assume a:"(1 \<le> length xs \<Longrightarrow> p01_1 xs def = x \<Longrightarrow> x \<in> set xs)"
+  assume b:"1 \<le> length (a # xs)"
+  assume c:" p01_1 (a # xs) def = x"
+  assume " xs = aa # list"
+  from this and a and b and c show  "x \<in> set (a # xs)" by simp
+ qed
 qed
 
 
 
 
-(*step by step syntactical replacement with Isar*)
-theorem isar_tp01_1_3 : fixes ls a b  shows "p01_1 ( ls @ [a]) b = a " 
-proof (induct ls)
- case Nil
-  have "p01_1 ([] @ [a]) b =  p01_1 [a] b" unfolding append_Nil ..  (*instead of   the two dots ".." one could write "by (rule refl)" *)(*instead of unfolding \<rightarrow> "by (subst append_Nil[where ?ys = "[a]"]; rule refl)" *)
-  also have "\<dots> = a" unfolding p01_1.simps(2) ..
-  finally show "p01_1 ([] @ [a]) b = a" . 
-next
- case (Cons  aa ls)
-  show " p01_1 (ls @ [a]) b = a \<Longrightarrow>  p01_1 ((aa # ls) @ [a]) b = a "
-  proof (cases ls)
-   case Nil
-    assume "ls = []" 
-    assume "p01_1 (ls @ [a]) b = a"
-    have " p01_1 ((aa # ls) @ [a]) b =  p01_1 (aa # ls @ [a]) b " unfolding append_Cons ..
-    also have "\<dots> = p01_1 (aa # [] @ [a]) b" unfolding \<open>ls = []\<close> ..
-    also have "\<dots> = p01_1 (aa # [a]) b" unfolding append_Nil ..
-    also have "\<dots> = p01_1 [a] b" unfolding p01_1.simps(3) ..
-    also have "\<dots> = a" unfolding p01_1.simps(2)  ..
-    finally show "p01_1 ((aa # ls) @ [a]) b = a" . 
-  next  
-   case (Cons ab list)
-    fix ab list 
-    assume IH:"p01_1 (ls @ [a]) b = a"
-    assume "ls = ab # list"
-
-    from  \<open>ls= ab # list\<close> and  IH have "p01_1 ((ab # list) @ [a]) b = a"  by (rule subst)
-    with append_Cons have  "p01_1 (ab # list @ [a]) b = a" by (rule subst)
-    note IH2 = this
-
-    have  "p01_1 ((aa # ls) @ [a]) b = p01_1 ((aa # ab # list)@ [a]) b" unfolding \<open>ls = ab # list\<close> ..
-    also have "\<dots> =  p01_1 (aa # (ab # list)@ [a]) b " unfolding append_Cons ..
-    also have "\<dots> =  p01_1 (aa # ab # list@ [a]) b" unfolding append_Cons ..
-    also have "\<dots> = p01_1 (ab # list @ [a]) b " unfolding p01_1.simps(3) ..
-    also have "\<dots> = a " unfolding IH2 ..
-    finally show " p01_1 ((aa # ls) @ [a]) b = a" .
-  qed
-qed
-
-
-(*on other way to proof this (less readable but probably easier to understand)*)
-theorem isar_tp01_1_4 : fixes ls a b  shows "p01_1 ( ls @ [a]) b = a " 
-proof (induct ls)
-{
-  show "p01_1 ([] @ [a]) b = a"
-  proof (subst append_Nil)
-  {
-    show " p01_1 [a] b = a"
-    proof (subst p01_1.simps(2))
-    {
-      show "a = a" by (rule refl)
-    }
-    qed
-  }
-  qed
-  fix aa ls
-  assume "p01_1 (ls @ [a]) b = a"
-  show " p01_1 ((aa # ls) @ [a]) b = a "
-  proof (cases ls)
-  {
-    assume "ls = []"
-    show "p01_1 ((aa # ls) @ [a]) b = a"
-    proof (subst \<open>ls=[]\<close>)
-    {
-      show "p01_1 ([aa] @ [a]) b = a"
-      proof (subst append_Cons)
-      {
-        show "p01_1 (aa # [] @ [a]) b = a"
-        proof (subst append_Nil)
-        {
-          show " p01_1 [aa, a] b = a"
-          proof (subst p01_1.simps(3))
-          {
-            show "p01_1 [a] b = a" 
-            proof (subst p01_1.simps(2))
-            {
-              show "a = a" by (rule refl)
-            }
-            qed
-          }
-          qed
-        }
-        qed
-      }
-      qed
-    }
-    qed
-  }
-  fix ab list
-  assume "ls = ab # list"
-  from this and  \<open>p01_1 (ls @ [a]) b = a\<close> have "p01_1 ((ab # list) @ [a]) b = a" by (rule subst) 
-  with append_Cons have "p01_1 (ab # list @ [a]) b = a" by (rule subst)
-  show "p01_1 ((aa # ls) @ [a]) b = a" 
-  proof (subst \<open>ls = ab # list\<close>)
-  {
-    show " p01_1 ((aa # ab # list) @ [a]) b = a "
-    proof (subst  append_Cons)
-    {
-      show "p01_1 (aa # (ab # list) @ [a]) b = a "
-      proof (subst append_Cons )
-      {
-        show "p01_1 (aa # ab # list @ [a]) b = a "
-        proof (subst p01_1.simps(3))
-        {
-          show "p01_1 (ab # list @ [a]) b = a " by (rule \<open>p01_1 (ab # list @ [a]) b = a\<close>)
-        }
-        qed
-      }
-      qed
-    }
-    qed
-  }
-  qed
-  qed
-}
-qed
-
-
-
-(*yet another way to prove the same theorem*)
-theorem isar_tp01_1_4 : fixes ls a b  shows "p01_1 ( ls @ [a]) b = a " 
-using [[simp_trace_new mode=full]]
-proof (induct ls)
-
-  have True by (rule TrueI)
-  hence "a = a" by simp  (*if one would want to use subst , one hab to use HOL.simp_thms (subst HOL.simp_thms(6)), which is strongly discouraged*)
-  hence  "p01_1 [a] b = a" by (subst p01_1.simps(2))
-  hence "p01_1 ([] @ [a]) b = a" by (subst append_Nil)
-  thus "p01_1 ([] @ [a]) b = a" .
- next
-  fix aa ls 
-  assume "p01_1 (ls @ [a]) b = a "
-  show "p01_1 ((aa # ls) @ [a]) b = a "
-  proof (cases ls)
-    have True by (rule TrueI)
-    hence "a = a" by simp
-    hence "p01_1 [a] b = a" by (subst p01_1.simps(2))
-    hence "p01_1 [a] b = a" by (subst p01_1.simps)
-
-
-(*from now on I will mix isar and apply-script proofs and I will also mix step-by-step solving with automation*)
-
-
-fun p01_2 :: "'a list \<Rightarrow> 'a option" where
+fun p01_2 :: "'a list \<Rightarrow> 'a option " where
 "p01_2 [] = None"|
 "p01_2 [x] = Some x"|
 "p01_2 (x#xs) = p01_2 xs"
 
 
-value "p01_2 [1,2,3,4,5] :: int option"
-value "p01_2 [] :: int option"
+value "p01_2 []"
 
-term p01_2
+value "p01_2 [1 , 2] :: int option"
 
+lemma "p01_2 [] = None" by simp
 
-lemma tp01_2_1 : "p01_2 [] = None"
-apply (rule p01_2.simps(1))
-done 
+lemma "p01_2 [x] = Some x" by simp
 
-lemma  isar_tp01_2_1 : "p01_2 [] = None"
-proof -
-show ?thesis by (rule p01_2.simps(1))
+lemma "p01_2 (xs @ [a]) = Some a" 
+proof (induct xs)
+  show " p01_2 ([] @ [a]) = Some a" by simp
+ next 
+  fix aa xs 
+  assume " p01_2 (xs @ [a]) = Some a"
+  thus "p01_2 ((aa # xs) @ [a]) = Some a " 
+  proof (cases xs)
+    assume "p01_2 (xs @ [a]) = Some a"
+    assume "xs = []"
+    thus " p01_2 ((aa # xs) @ [a]) = Some a" by simp
+   next 
+    fix ab list 
+    assume " p01_2 (xs @ [a]) = Some a"
+    moreover
+    assume "xs = ab # list"
+    ultimately show "p01_2 ((aa # xs) @ [a]) = Some a" by simp
+  qed
 qed
 
+lemma "p01_2 ls = Some x \<Longrightarrow> last ls = x"
+proof (induct ls)
+  show "p01_2 [] = Some x \<Longrightarrow> last [] = x" by simp
+ next 
+  fix a ls
+  show " (p01_2 ls = Some x \<Longrightarrow> last ls = x) \<Longrightarrow> p01_2 (a # ls) = Some x \<Longrightarrow> last (a # ls) = x "
+  proof (cases ls)
+    assume " (p01_2 ls = Some x \<Longrightarrow> last ls = x)"
+    assume a:" p01_2 (a # ls) =  Some x"
+    assume " ls = []"
+    with a show "last (a # ls) = x" by simp
+   next 
+    fix aa list 
+    assume a:"(p01_2 ls = Some x \<Longrightarrow> last ls = x)"
+    assume b:"p01_2 (a # ls) = Some x"
+    assume " ls = aa # list"
+    with a and b show "last (a # ls) = x" by simp
+  qed
+qed
 
-lemma 
+ 
