isabelleSrc/P03.thy
@@ -1,0 +1,11 @@
+theory P03
+imports Main 
+begin 
+
+
+
+fun p03_1 :: "'a list \<Rightarrow> nat \<Rightarrow> 'a option" where
+"p03_1 [] _ = None"|
+"p03_1 (x#xs) n = (if n = 1 then Some x else  p03_1 xs (n - 1))"
+
+value "p03_1 [1,2 ,3,4] 3 :: int option"
